mrdts/Observed-remove_set_eff/App.fst
@@ -219,24 +219,28 @@ let rc_intermediate2 (l l' a b:concrete_st) (o1 o2 o o':op_t)
                     eq (merge l (do a o') (do b o)) (do (do l' o) o'))
           (ensures eq (merge (do l o') (do (do a o') o1) (do (do (do b o) o') o2)) (do (do (do (do l' o) o') o1) o2)) = admit()
 
-let rc_intermediate2' (l l' a b:concrete_st) (o1 o2 o o':op_t)
- : Lemma (requires distinct_ops o1 o2 /\ Rem? (snd (snd o1)) /\ Add? (snd (snd o2)) /\ get_ele o1 = get_ele o2 /\ //Fst_then_snd? (rc o1 o2) /\ 
-                    distinct_ops o o' /\ Rem? (snd (snd o)) /\ Add? (snd (snd o')) /\ get_ele o = get_ele o' /\ //Fst_then_snd? (rc o o') /\
-                    get_rid o' = get_rid o2 /\
-                    eq (merge l (do a o1) (do b o2)) (do (do l' o1) o2) /\ 
-                    eq (merge l (do a o') (do b o)) (do (do l' o) o'))
-          (ensures eq (merge (do l o') (do (do a o') o1) (do (do (do b o) o') o2)) (do (do (do (do l' o) o') o1) o2)) = 
-  if get_ele o' = get_ele o2 then () else ()
-  
-let rc_intermediate2'' (l l' a b:concrete_st) (o1 o2 o o':op_t)
- : Lemma (requires distinct_ops o1 o2 /\ Rem? (snd (snd o1)) /\ Add? (snd (snd o2)) /\ get_ele o1 = get_ele o2 /\ //Fst_then_snd? (rc o1 o2) /\ 
-                    distinct_ops o o' /\ Rem? (snd (snd o)) /\ Add? (snd (snd o')) /\ get_ele o = get_ele o' /\ //Fst_then_snd? (rc o o') /\
-                    eq (merge l (do a o1) (do b o2)) (do (do l' o1) o2) /\
-                    eq (merge l (do a o') (do b o)) (do (do l' o) o') /\
-                    eq (merge (do l o') (do (do a o') o1) (do (do b o') o2)) (do (do (do l' o') o1) o2))
-          (ensures eq (merge (do l o') (do (do a o') o1) (do (do (do b o) o') o2)) (do (do (do (do l' o) o') o1) o2)) = 
- if get_ele o' = get_ele o2 then () else ()
-          
+let comm_intermediate1' (l:concrete_st) (o1 o2 o o' o3:op_t)
+  : Lemma (requires distinct_ops o1 o2 /\ Either? (rc o1 o2) /\
+                    distinct_ops o o' /\ Fst_then_snd? (rc o o') /\
+                    distinct_ops o' o1 /\ distinct_ops o' o2 /\ distinct_ops o3 o1 /\ 
+                    eq (do (do l o2) o1) (do (do l o1) o2) /\
+                    ~ (exists o3 a'. eq (do l o1) (do a' o3) /\ distinct_ops o2 o3 /\ Fst_then_snd? (rc o2 o3)) /\
+                    ~ (exists o3 b'. eq (do l o2) (do b' o3) /\ distinct_ops o1 o3 /\ Fst_then_snd? (rc o1 o3)))
+          (ensures (eq (merge l (do l o1) (do l o2)) (do (do l o1) o2) /\
+                    eq (merge (do l o') (do (do l o') o1) (do (do (do l o) o') o2)) (do (do (do (do l o) o') o1) o2)) ==>
+      eq (merge (do (do l o3) o') (do (do (do l o3) o') o1) (do (do (do (do l o3) o) o') o2)) (do (do (do (do (do l o3) o) o') o1) o2)) = ()
+
+let comm_intermediate1'' (l:concrete_st) (o1 o2 o o' o3:op_t)
+  : Lemma (requires distinct_ops o1 o2 /\ Either? (rc o1 o2) /\
+                    distinct_ops o o' /\ Fst_then_snd? (rc o o') /\
+                    distinct_ops o' o1 /\ distinct_ops o' o2 /\ distinct_ops o3 o1 /\ 
+                    eq (do (do l o2) o1) (do (do l o1) o2) /\
+                    ~ (exists o3 a'. eq (do l o1) (do a' o3) /\ distinct_ops o2 o3 /\ Fst_then_snd? (rc o2 o3)) /\
+                    ~ (exists o3 b'. eq (do l o2) (do b' o3) /\ distinct_ops o1 o3 /\ Fst_then_snd? (rc o1 o3)))
+          (ensures (eq (merge l (do l o1) (do l o2)) (do (do l o2) o1) /\
+                    eq (merge (do l o') (do (do l o') o1) (do (do (do l o) o') o2)) (do (do (do (do l o) o') o2) o1)) ==>
+      eq (merge (do (do l o3) o') (do (do (do l o3) o') o1) (do (do (do (do l o3) o) o') o2)) (do (do (do (do (do l o3) o) o') o2) o1)) = ()
+      
 let comm_intermediate1 (l:concrete_st) (o1 o2 o o' o3:op_t)
   : Lemma (requires distinct_ops o1 o2 /\ Either? (rc o1 o2) /\
                     distinct_ops o o' /\ Fst_then_snd? (rc o o') /\
@@ -249,7 +253,9 @@ let comm_intermediate1 (l:concrete_st) (o1 o2 o o' o3:op_t)
       eq (merge (do (do l o3) o') (do (do (do l o3) o') o1) (do (do (do (do l o3) o) o') o2)) (do (do (do (do (do l o3) o) o') o1) o2)) /\
                    ((eq (merge l (do l o1) (do l o2)) (do (do l o2) o1) /\
                      eq (merge (do l o') (do (do l o') o1) (do (do (do l o) o') o2)) (do (do (do (do l o) o') o2) o1)) ==>
-      eq (merge (do (do l o3) o') (do (do (do l o3) o') o1) (do (do (do (do l o3) o) o') o2)) (do (do (do (do (do l o3) o) o') o2) o1))) = ()
+      eq (merge (do (do l o3) o') (do (do (do l o3) o') o1) (do (do (do (do l o3) o) o') o2)) (do (do (do (do (do l o3) o) o') o2) o1))) = 
+   comm_intermediate1' l o1 o2 o o' o3;
+   comm_intermediate1'' l o1 o2 o o' o3
 
 let comm_intermediate2 (l l' a b:concrete_st) (o1 o2 o o':op_t)
   : Lemma (requires distinct_ops o1 o2 /\ Either? (rc o1 o2) /\ 
